proof structure for ZF deduction

theories/Reductions/BPCP_to_ZFD.v
@@ -28,8 +28,8 @@ Definition ZF phi :=
   \/ phi = ax_power
   \/ phi = ax_om1
   \/ phi = ax_om2
-  \/ (bounded 1 phi /\ phi = ax_sep phi)
-  \/ (bounded 2 phi /\ phi = ax_rep phi).
+  \/ (exists psi, bounded 1 psi /\ phi = ax_sep psi)
+  \/ (exists psi, bounded 2 psi /\ phi = ax_rep psi).
 
 
 
@@ -54,21 +54,214 @@ Proof.
   apply IE with phi; eauto using Weak.
 Qed.
 
+Lemma prv_T_ExI (p : peirce) (b : bottom) T phi t :
+  T ⊩ phi[t..] -> T ⊩ ∃ phi.
+Proof.
+  intros [A[A1 A2]]. use_theory A.
+  now apply ExI with t.
+Qed.
+
+Lemma prv_T_CI (p : peirce) (b : bottom) T phi psi :
+  T ⊩ phi -> T ⊩ psi -> T ⊩ (phi ∧ psi).
+Proof.
+  intros [A[A1 A2]] [B[B1 B2]]. use_theory (A++B).
+   apply CI; eauto using Weak.
+Qed.
+
+Lemma pair_el x y z :
+  ZF ⊩IE (z ≡ x ∨ z ≡ y) --> z ∈ {x; y}.
+Proof.
+Admitted.
+
 Lemma bunion_el x y z :
-  ZF ⊩IE ((z ∈ x ∨ z ∈ y) --> z ∈ x ∪ y).
+  ZF ⊩IE (z ∈ x ∨ z ∈ y) --> z ∈ x ∪ y.
 Proof.
   apply prv_T_impl.
+Admitted.
   
 
-Theorem stack_enc_spec R s t :
+Lemma enc_stack_spec R s t :
   s/t el R -> ZF ⊩IE opair (enc_string s) (enc_string t) ∈ enc_stack R.
 Proof.
   induction R as [|[u v] IH]; cbn; auto.
   intros [[=]| H]; subst.
-  - oapply 
+  - admit.
+Admitted.
 
-Theorem BPCP_slv R :
-  BPCP R -> ZF ⊩IE solvable R.
+Fixpoint tnumeral n :=
+  match n with 
+  | O => ∅
+  | S n => σ (tnumeral n)
+  end.
+
+Fixpoint enc_derivations B n :=
+  match n with 
+  | O => sing (opair ∅ (enc_stack B))
+  | S n => enc_derivations B n ∪ sing (opair (tnumeral (S n)) (enc_stack (derivations B (S n))))
+  end.
+
+Lemma substt_bounded0 t sigma :
+  bounded_term 0 t -> subst_term sigma t = t.
 Proof.
+  induction 1; cbn.
+  - lia.
+  - f_equal. erewrite <- vec_id. 2: reflexivity.
+    apply vec_map_ext. apply H0.
+Qed.
+
+Lemma subst_bounded0 phi sigma :
+  bounded 0 phi -> phi[sigma] = phi.
+Proof.
+  remember 0 as n.
+  induction 1; cbn; subst; try firstorder congruence.
+  - f_equal. erewrite <- vec_id. 2: reflexivity.
+    apply vec_map_ext. intros x H'. now apply substt_bounded0, H.
+  - admit.
+Admitted.
+
+Ltac solve_bounds :=
+  repeat constructor; try lia; try inversion X; intros;
+  match goal with
+  | H : vec_in ?x (Vector.cons ?y ?v) |- _ => repeat apply vec_cons_inv in H as [->|H]; try inversion H
+  | _ => idtac
+  end.
+
+Lemma bounded_term_up t n k :
+  bounded_term n t -> k >= n -> bounded_term k t.
+Proof.
+Admitted.
+
+Lemma bounded_up phi n k :
+  bounded n phi -> k >= n -> bounded k phi.
+Proof.
+Admitted.
+
+Lemma ZF_bounded phi :
+  ZF phi -> bounded 0 phi.
+Proof.
+  intros [->|[->|[->|[->|[->|[->|[->|[[psi [H ->]]|[psi [H ->]]]]]]]]]];
+  repeat solve_bounds; eauto using bounded_up.
+  - admit.
+  - admit.
+Admitted.
+
+Lemma ZF_all phi :
+  ZF ⊩IE phi -> ZF ⊩IE ∀ phi.
+Proof.
+  intros [A[H1 H2]]. use_theory A. apply AllI.
+  enough ([psi[form_shift] | psi ∈ A] = A) as -> by trivial.
+  erewrite <- list_id. 2: reflexivity.
+  apply map_ext_in. intros psi H % H1.
+  apply subst_bounded0, ZF_bounded, H.
+Qed.
+
+Lemma prv_T_CE1 (p : peirce) (b : bottom) T phi psi :
+  T ⊩ (phi ∧ psi) -> T ⊩ phi.
+Proof.
+Admitted.
+
+Lemma prv_T_CE2 (p : peirce) (b : bottom) T phi psi :
+  T ⊩ (phi ∧ psi) -> T ⊩ psi.
+Proof.
+Admitted.
+
+Lemma prv_T_AllE (p : peirce) (b : bottom) T phi t :
+  (T ⊩ ∀ phi) -> T ⊩ phi[t..].
+Proof.
+  intros [A[H1 H2]]. use_theory A. now apply AllE.
+Qed.
+
+Lemma ZF_numeral n :
+  ZF ⊩IE tnumeral n ∈ ω.
+Proof.
+  induction n; cbn.
+  - eapply prv_T_CE1. apply elem_prv.
+    do 5 right. left. reflexivity.
+  - eapply prv_T_mp; try apply IHn.
+    change (ZF ⊩IE ($0 ∈ ω --> σ ($0) ∈ ω)[(tnumeral n)..]).
+    apply prv_T_AllE. eapply prv_T_CE2. apply elem_prv.
+    do 5 right. left. reflexivity.
+Qed.
+
+Lemma enc_derivations_base R n :
+  ZF ⊩IE {{∅; ∅}; {∅; enc_stack R}} ∈ enc_derivations R n.
+Proof.
+Admitted.
+
+Lemma perst_bounded0 t sigma :
+  bounded_term 0 t -> bounded_term 0 (subst_term sigma t).
+Proof.
+  intros H. now rewrite substt_bounded0.
+Qed.
+
+Lemma enc_bool_bounded0 b :
+  bounded_term 0 (enc_bool b).
+Proof.
+  destruct b; repeat solve_bounds.
+Qed.
+
+Lemma prep_string_bounded s t n :
+  bounded_term n t -> bounded_term n (prep_string s t).
+Proof.
+  induction s; cbn; repeat solve_bounds; eauto.
+  all: eapply bounded_term_up; try apply enc_bool_bounded0; lia.
+Qed.
+
+Lemma enc_string_bounded0 s :
+  bounded_term 0 (enc_string s).
+Proof.
+  apply prep_string_bounded. repeat solve_bounds.
+Qed.
+
+Lemma tnumeral_bounded0 n :
+  bounded_term 0 (tnumeral n).
+Proof.
+  induction n; cbn; repeat solve_bounds; try inversion X; trivial.
+Qed.
+
+Hint Resolve tnumeral_bounded0.
+
+Lemma enc_stack_bounded0 B :
+  bounded_term 0 (enc_stack B).
+Proof.
+  induction B as [|[]IH]; cbn; repeat solve_bounds; eauto using enc_string_bounded0.
+Qed.
+
+Hint Resolve enc_stack_bounded0.
+
+Lemma enc_derivations_bounded0 B n :
+  bounded_term 0 (enc_derivations B n).
+Proof.
+  induction n; cbn; repeat solve_bounds; eauto.
+Qed.
+
+Hint Resolve enc_string_bounded0 enc_derivations_bounded0.
+
+Theorem BPCP_slv B :
+  BPCP B -> ZF ⊩IE solvable B.
+Proof.
+  intros [s H] % BPCP_BPCP'. destruct (derivable_derivations H) as [n Hn].
+
+  (* enough (ZF ⊩IE (tnumeral n) ∈ ω
+          ∧ function' (enc_derivations R n)
+          ∧ solutions R (enc_derivations R n) (tnumeral n)
+          ∧ opair (tnumeral n) (enc_stack (derivations R n)) ∈ (enc_derivations R n)
+          ∧ (opair (enc_string s) (enc_string s)) ∈ (enc_stack (derivations R n))
+          ∧ (opair (enc_string s) (enc_string s)) ≡ opair (enc_string s) (enc_string s)). *)
+
+  apply prv_T_ExI with (tnumeral n);
+  apply prv_T_ExI with (enc_derivations B n);
+  apply prv_T_ExI with (opair (enc_string s) (enc_string s));
+  apply prv_T_ExI with (enc_string s);
+  apply prv_T_ExI with (enc_stack (derivations B n)); fold subst_form.
+  cbn; rewrite !substt_bounded0; repeat apply perst_bounded0; eauto.
+  repeat apply prv_T_CI.
+  - apply ZF_numeral.
+  - repeat apply ZF_all. asimpl. admit.
+  - apply enc_derivations_base.
+  - repeat apply ZF_all. admit.
+  - admit.
+  - now apply enc_stack_spec.
+  - admit.
 Admitted.
 
